Veir/IR/Buffed/Bounds.lean
@@ -1,0 +1,200 @@
+
+instance : HAdd Nat (Std.Rco Int) (Std.Rco Int) where
+  hAdd x y := (x + y.lower)...(x + y.upper)
+
+section in_bounds
+variable [HasOpInfo OpInfo]
+
+/-! ## ValueImpl -/
+
+section value_impl
+
+def ValueImplMPtr.range (ptr : ValueImplMPtr) :=
+  ptr.toNat + ValueImpl.range
+
+@[grind]
+def ValueImplMPtr.InBoundsBytes (ptr : ValueImplMPtr) (bctx : IRContext OpInfo) :=
+  IsIncludedIN ptr.range bctx.mem.range
+
+@[grind, inline]
+def ValueImplOPtr.isNone (optr : ValueImplOPtr) := optr = (-1 : UInt64)
+
+@[grind, inline]
+def ValueImplOPtr.toM (optr : ValueImplOPtr) : ValueImplMPtr := optr
+
+@[grind]
+def ValueImplOPtr.InBoundsBytes (ptr : ValueImplOPtr) (bctx : IRContext OpInfo) : Prop :=
+  (¬ ptr.isNone) → ptr.toM.InBoundsBytes bctx
+
+end value_impl
+
+/-! ## OpResult -/
+
+section op_result
+
+def OpResultMPtr.range (ptr : OpResultMPtr) :=
+  ptr.toNat + OpResult.range
+
+@[grind]
+def OpResultMPtr.InBoundsBytes (ptr : OpResultMPtr) (bctx : IRContext OpInfo) :=
+  IsIncludedIN ptr.range bctx.mem.range
+
+@[grind, inline]
+def OpResultOPtr.isNone (optr : OpResultOPtr) := optr = (-1 : UInt64)
+
+@[grind, inline]
+def OpResultOPtr.toM (optr : OpResultOPtr) : OpResultMPtr := optr
+
+@[grind]
+def OpResultOPtr.InBoundsBytes (ptr : OpResultOPtr) (bctx : IRContext OpInfo) : Prop :=
+  (¬ ptr.isNone) → ptr.toM.InBoundsBytes bctx
+
+end op_result
+
+/-! ## BlockArgument -/
+
+section block_argument
+
+def BlockArgumentMPtr.range (ptr : BlockArgumentMPtr) :=
+  ptr.toNat + BlockArgument.range
+
+@[grind]
+def BlockArgumentMPtr.InBoundsBytes (ptr : BlockArgumentMPtr) (bctx : IRContext OpInfo) :=
+  IsIncludedIN ptr.range bctx.mem.range
+
+@[grind, inline]
+def BlockArgumentOPtr.isNone (optr : BlockArgumentOPtr) := optr = (-1 : UInt64)
+
+@[grind, inline]
+def BlockArgumentOPtr.toM (optr : BlockArgumentOPtr) : BlockArgumentMPtr := optr
+
+@[grind]
+def BlockArgumentOPtr.InBoundsBytes (ptr : BlockArgumentOPtr) (bctx : IRContext OpInfo) : Prop :=
+  (¬ ptr.isNone) → ptr.toM.InBoundsBytes bctx
+
+end block_argument
+
+/-! ## OpOperand -/
+
+section op_operand
+
+def OpOperandMPtr.range (ptr : OpOperandMPtr) :=
+  ptr.toNat + OpOperand.range
+
+@[grind]
+def OpOperandMPtr.InBoundsBytes (ptr : OpOperandMPtr) (bctx : IRContext OpInfo) :=
+  IsIncludedIN ptr.range bctx.mem.range
+
+@[grind, inline]
+def OpOperandOPtr.isNone (optr : OpOperandOPtr) := optr = (-1 : UInt64)
+
+@[grind, inline]
+def OpOperandOPtr.toM (optr : OpOperandOPtr) : OpOperandMPtr := optr
+
+@[grind]
+def OpOperandOPtr.InBoundsBytes (ptr : OpOperandOPtr) (bctx : IRContext OpInfo) : Prop :=
+  (¬ ptr.isNone) → ptr.toM.InBoundsBytes bctx
+
+end op_operand
+
+/-! ## BlockOperand -/
+
+section block_operand
+
+def BlockOperandMPtr.range (ptr : BlockOperandMPtr) :=
+  ptr.toNat + BlockOperand.range
+
+@[grind]
+def BlockOperandMPtr.InBoundsBytes (ptr : BlockOperandMPtr) (bctx : IRContext OpInfo) :=
+  IsIncludedIN ptr.range bctx.mem.range
+
+@[grind, inline]
+def BlockOperandOPtr.isNone (optr : BlockOperandOPtr) := optr = (-1 : UInt64)
+
+@[grind, inline]
+def BlockOperandOPtr.toM (optr : BlockOperandOPtr) : BlockOperandMPtr := optr
+
+@[grind]
+def BlockOperandOPtr.InBoundsBytes (ptr : BlockOperandOPtr) (bctx : IRContext OpInfo) : Prop :=
+  (¬ ptr.isNone) → ptr.toM.InBoundsBytes bctx
+
+end block_operand
+
+/-! ## Operation -/
+
+section operation
+
+@[grind]
+def OperationMPtr.toH (ptr : OperationMPtr) : OperationPtr := ⟨ptr.toNat⟩
+
+def OperationMPtr.range (ptr : OperationMPtr) (ctx : Veir.IRContext OpInfo) (ib : ptr.toH.InBounds ctx := by grind) :=
+  ptr.toNat + Operation.range ptr.toH ctx ib
+
+@[grind]
+def OperationMPtr.InBoundsBytes (ptr : OperationMPtr) (op : OperationPtr)
+    (ctx : Veir.IRContext OpInfo) (ib : op.InBounds ctx) (bctx : IRContext OpInfo) :=
+  IsIncludedIN (OperationMPtr.range ptr op ctx ib) bctx.mem.range
+
+@[grind, inline]
+def OperationOPtr.isNone (optr : OperationOPtr) := optr = (-1 : UInt64)
+
+@[grind, inline]
+def OperationOPtr.toM (optr : OperationOPtr) : OperationMPtr := optr
+
+@[grind]
+def OperationOPtr.InBoundsBytes (ptr : OperationOPtr) (op : OperationPtr)
+    (ctx : Veir.IRContext OpInfo) (ib : op.InBounds ctx) (bctx : IRContext OpInfo) : Prop :=
+  (¬ ptr.isNone) → OperationMPtr.InBoundsBytes (OperationOPtr.toM ptr) op ctx ib bctx
+
+end operation
+
+/-! ## Block -/
+
+section block
+
+def BlockMPtr.range (ptr : BlockMPtr) (bl : BlockPtr)
+    (ctx : Veir.IRContext OpInfo) (ib : bl.InBounds ctx) :=
+  ptr.toNat + Block.range bl ctx ib
+
+@[grind]
+def BlockMPtr.InBoundsBytes (ptr : BlockMPtr) (bl : BlockPtr)
+    (ctx : Veir.IRContext OpInfo) (ib : bl.InBounds ctx) (bctx : IRContext OpInfo) :=
+  IsIncludedIN (ptr.range bl ctx ib) bctx.mem.range
+
+@[grind, inline]
+def BlockOPtr.isNone (optr : BlockOPtr) := optr = (-1 : UInt64)
+
+@[grind, inline]
+def BlockOPtr.toM (optr : BlockOPtr) : BlockMPtr := optr
+
+@[grind]
+def BlockOPtr.InBoundsBytes (ptr : BlockOPtr) (bl : BlockPtr)
+    (ctx : Veir.IRContext OpInfo) (ib : bl.InBounds ctx) (bctx : IRContext OpInfo) : Prop :=
+  (¬ ptr.isNone) → BlockMPtr.InBoundsBytes (BlockOPtr.toM ptr) bl ctx ib bctx
+
+end block
+
+/-! ## Region -/
+
+section region
+
+def RegionMPtr.range (ptr : RegionMPtr) :=
+  ptr.toNat + Region.range
+
+@[grind]
+def RegionMPtr.InBoundsBytes (ptr : RegionMPtr) (bctx : IRContext OpInfo) :=
+  IsIncludedIN ptr.range bctx.mem.range
+
+@[grind, inline]
+def RegionOPtr.isNone (optr : RegionOPtr) := optr = (-1 : UInt64)
+
+@[grind, inline]
+def RegionOPtr.toM (optr : RegionOPtr) : RegionMPtr := optr
+
+@[grind]
+def RegionOPtr.InBoundsBytes (ptr : RegionOPtr) (bctx : IRContext OpInfo) : Prop :=
+  (¬ ptr.isNone) → ptr.toM.InBoundsBytes bctx
+
+end region
+
+end in_bounds
