Veir/IR/Buffed/Layout.lean
@@ -1,0 +1,223 @@
+module
+
+public import Veir.IR.Basic
+
+/-! # Sizes of the different fields, in bytes. -/
+
+public section
+
+instance : HAdd UInt64 Int64 UInt64 where
+  hAdd x y := x.toInt64 + y |>.toUInt64
+instance : HAdd Int64 UInt64 Int64 where
+  hAdd x y := x + y.toInt64
+
+theorem UInt64.add_int64_pos (x : UInt64) (y : Int64) : (x + y).toNat = x.toNat + y.toInt := by
+  sorry
+
+namespace Veir.Buffed
+
+abbrev ptrSize : UInt64 := 8
+abbrev countSize : UInt64 := 8
+
+namespace ValueImpl
+namespace Sizes
+abbrev type : UInt64 := ptrSize
+abbrev firstUse : UInt64 := ptrSize
+end Sizes
+abbrev size : UInt64 := ValueImpl.Sizes.type + ValueImpl.Sizes.firstUse
+end ValueImpl
+
+namespace OpResult
+namespace Sizes
+abbrev index : UInt64 := ptrSize
+abbrev owner : UInt64 := ptrSize
+end Sizes
+abbrev size : UInt64 := ValueImpl.size + Sizes.index + Sizes.owner
+end OpResult
+
+namespace BlockArgument
+namespace Sizes
+abbrev index : UInt64 := ptrSize
+abbrev loc : UInt64 := 0
+abbrev owner : UInt64 := ptrSize
+end Sizes
+abbrev size : UInt64 := ValueImpl.size + Sizes.index + Sizes.loc + Sizes.owner
+end BlockArgument
+
+namespace OpOperand
+namespace Sizes
+abbrev nextUse : UInt64 := ptrSize
+abbrev back : UInt64 := ptrSize
+abbrev owner : UInt64 := ptrSize
+abbrev value : UInt64 := ptrSize
+end Sizes
+abbrev size : UInt64 := Sizes.nextUse + Sizes.back + Sizes.owner + Sizes.value
+end OpOperand
+
+namespace BlockOperand
+namespace Sizes
+abbrev nextUse : UInt64 := ptrSize
+abbrev back : UInt64 := ptrSize
+abbrev owner : UInt64 := ptrSize
+abbrev value : UInt64 := ptrSize
+end Sizes
+abbrev size : UInt64 := Sizes.nextUse + Sizes.back + Sizes.owner + Sizes.value
+end BlockOperand
+
+namespace Operation
+variable [HasOpInfo OpInfo] (op : OperationPtr) (ctx : IRContext OpInfo)
+
+-- Add this info to the typeclasses
+def propertySize (opCode : OpInfo) : UInt64 := sorry
+@[inline] abbrev opInfoSize : Nat := 4
+def decodeOpInfo (x : UInt32) : OpInfo := sorry
+
+namespace Sizes
+abbrev results : UInt64 := UInt64.ofNat (op.getNumResults! ctx) * OpResult.size
+abbrev numResults : UInt64 := countSize
+abbrev prev : UInt64 := ptrSize
+abbrev next : UInt64 := ptrSize
+abbrev parent : UInt64 := ptrSize
+abbrev opType : UInt64 := UInt64.ofNat opInfoSize
+abbrev attrs : UInt64 := ptrSize
+abbrev properties : UInt64 := propertySize (op.getOpType! ctx)
+abbrev numBlockOperands : UInt64 := countSize
+abbrev blockOperands : UInt64 := UInt64.ofNat (op.getNumSuccessors! ctx) * BlockOperand.size
+abbrev numRegions : UInt64 := countSize
+abbrev regions : UInt64 := UInt64.ofNat (op.getNumRegions! ctx) * ptrSize
+abbrev numOperands : UInt64 := countSize
+abbrev operands : UInt64 := UInt64.ofNat (op.getNumOperands! ctx) * BlockOperand.size
+end Sizes
+abbrev size : UInt64 :=
+  Sizes.results op ctx + Sizes.numResults + Sizes.prev + Sizes.next + Sizes.parent + Sizes.opType + Sizes.attrs +
+  Sizes.properties op ctx + Sizes.numBlockOperands + Sizes.blockOperands op ctx +
+  Sizes.numRegions + Sizes.regions op ctx + Sizes.numBlockOperands + Sizes.operands op ctx
+end Operation
+
+namespace Block
+variable [HasOpInfo OpInfo] (bl : BlockPtr) (ctx : IRContext OpInfo)
+namespace Sizes
+abbrev firstUse : UInt64 := ptrSize
+abbrev prev : UInt64 := ptrSize
+abbrev next : UInt64 := ptrSize
+abbrev parent : UInt64 := ptrSize
+abbrev firstOp : UInt64 := ptrSize
+abbrev lastOp : UInt64 := ptrSize
+abbrev numArguments : UInt64 := countSize
+abbrev arguments : UInt64 := UInt64.ofNat (bl.getNumArguments! ctx) * BlockArgument.size
+end Sizes
+
+abbrev size : UInt64 :=
+  Sizes.firstUse + Sizes.prev + Sizes.next + Sizes.parent + Sizes.firstOp + Sizes.lastOp +
+  Sizes.numArguments + Sizes.arguments bl ctx
+end Block
+
+namespace Region
+namespace Sizes
+abbrev firstBlock : UInt64 := ptrSize
+abbrev lastBlock : UInt64 := ptrSize
+abbrev parent : UInt64 := ptrSize
+end Sizes
+
+abbrev size : UInt64 := Sizes.firstBlock + Sizes.lastBlock + Sizes.parent
+end Region
+
+/-! # Offset of the different fields. -/
+
+namespace ValueImpl
+namespace Offsets
+abbrev type : Int64 := 0
+abbrev firstUse : Int64 := type + Sizes.type
+abbrev after : Int64 := firstUse + Sizes.firstUse
+end Offsets
+abbrev range : Std.Rco Int := 0...Offsets.after.toInt
+end ValueImpl
+
+namespace OpResult
+namespace Offsets
+abbrev index : Int64 := (0 : Int64) + ValueImpl.size
+abbrev owner : Int64 := index + Sizes.index
+abbrev after : Int64 := owner + Sizes.owner
+end Offsets
+abbrev range : Std.Rco Int := 0...Offsets.after.toInt
+end OpResult
+
+namespace BlockArgument
+namespace Offsets
+abbrev index : Int64 := (0 : Int64) + ValueImpl.size
+abbrev loc : Int64 := index + Sizes.index
+abbrev owner : Int64 := loc + Sizes.loc
+abbrev after : Int64 := owner + Sizes.owner
+end Offsets
+abbrev range : Std.Rco Int := 0...Offsets.after.toInt
+end BlockArgument
+
+namespace OpOperand
+namespace Offsets
+abbrev nextUse : Int64 := 0
+abbrev back : Int64 := nextUse + Sizes.nextUse
+abbrev owner : Int64 := back + Sizes.back
+abbrev value : Int64 := owner + Sizes.owner
+abbrev after : Int64 := value + Sizes.value
+end Offsets
+abbrev range : Std.Rco Int := 0...Offsets.after.toInt
+end OpOperand
+
+namespace BlockOperand
+namespace Offsets
+abbrev nextUse : Int64 := 0
+abbrev back : Int64 := nextUse + Sizes.nextUse
+abbrev owner : Int64 := back + Sizes.back
+abbrev value : Int64 := owner + Sizes.owner
+abbrev after : Int64 := value + Sizes.value
+end Offsets
+abbrev range : Std.Rco Int := 0...Offsets.after.toInt
+end BlockOperand
+
+namespace Operation
+variable [HasOpInfo OpInfo] (op : OperationPtr) (ctx : IRContext OpInfo)
+namespace Offsets
+abbrev results : Int64 := -((0 : Int64) + Sizes.results op ctx)
+abbrev numResults : Int64 := 0
+abbrev prev : Int64 := Offsets.numResults + Sizes.numResults
+abbrev next : Int64 := Offsets.prev + Sizes.prev
+abbrev parent : Int64 := Offsets.next + Sizes.next
+abbrev opType : Int64 :=  Offsets.parent + Sizes.parent
+abbrev numBlockOperands : Int64 := Offsets.opType + Sizes.opType
+abbrev numRegions : Int64 := Offsets.numBlockOperands + Sizes.numBlockOperands
+abbrev numOperands : Int64 := Offsets.numRegions + Sizes.numRegions
+abbrev attrs : Int64 := Offsets.numOperands + Sizes.numOperands
+abbrev properties : Int64 := Offsets.attrs + Sizes.attrs
+abbrev operands : Int64 := Offsets.properties + Sizes.properties op ctx
+abbrev blockOperands : Int64 := Offsets.operands op ctx + Sizes.operands op ctx
+abbrev regions : Int64 := Offsets.blockOperands op ctx + Sizes.blockOperands op ctx
+abbrev after : Int64 := Offsets.regions op ctx + Sizes.regions op ctx
+end Offsets
+abbrev range : Std.Rco Int := (Offsets.results op ctx).toInt...(Offsets.after op ctx).toInt
+end Operation
+
+namespace Block
+variable [HasOpInfo OpInfo] (bl : BlockPtr) (ctx : IRContext OpInfo)
+namespace Offsets
+abbrev firstUse : Int64 := 0
+abbrev prev : Int64 := firstUse + Sizes.firstUse
+abbrev next : Int64 := prev + Sizes.prev
+abbrev parent : Int64 := next + Sizes.next
+abbrev firstOp : Int64 := parent + Sizes.parent
+abbrev lastOp : Int64 := firstOp + Sizes.firstOp
+abbrev numArguments : Int64 := lastOp + Sizes.lastOp
+abbrev arguments : Int64 := numArguments + Sizes.numArguments
+abbrev after : Int64 := arguments + Sizes.arguments bl ctx
+end Offsets
+abbrev range : Std.Rco Int := 0...(Offsets.after bl ctx).toInt
+end Block
+
+namespace Region
+namespace Offsets
+abbrev firstBlock : Int64 := 0
+abbrev lastBlock : Int64 := firstBlock + Sizes.firstBlock
+abbrev parent : Int64 := lastBlock + Sizes.lastBlock
+abbrev after : Int64 := parent + Sizes.parent
+end Offsets
+abbrev range : Std.Rco Int := 0...Offsets.after.toInt
+end Region
