Veir/IR/Buffed/Sim.lean
@@ -1,0 +1,384 @@
+module
+
+public import Veir.IR.Buffed.RawAccessors
+public import Veir.IR.Buffed.Layout
+public import Veir.Prelude
+
+open Veir.Buffed
+
+-- TODO: Move in prelude?
+instance : HAdd Nat (Std.Rco Int) (Std.Rco Nat) where
+  hAdd x y := (x + y.lower).toNat...(x + y.upper).toNat
+
+namespace Veir
+
+variable [HasOpInfo OpInfo]
+
+/-! ## Translate a high-level pointer to a flat address. -/
+
+def OperationPtr.toFlat (ptr : OperationPtr) := ptr.id
+
+def BlockPtr.toFlat (ptr : BlockPtr) := ptr.id
+
+def RegionPtr.toFlat (ptr : RegionPtr) := ptr.id
+
+def OpResultPtr.toFlat (ptr : OpResultPtr) (ctx : IRContext OpInfo) :=
+  (Int.ofNat ptr.op.toFlat + (Buffed.Operation.Offsets.results (ptr.op.get! ctx)).toInt).toNat +
+  ptr.index * Buffed.OpResult.size.toNat
+
+def OpOperandPtr.toFlat (ptr : OpOperandPtr) (ctx : IRContext OpInfo) :=
+  (Int.ofNat ptr.op.toFlat + (Buffed.Operation.Offsets.operands (ptr.op.get! ctx)).toInt).toNat +
+  ptr.index * Buffed.OpOperand.size.toNat
+
+def BlockOperandPtr.toFlat (ptr : BlockOperandPtr) (ctx : IRContext OpInfo) :=
+  (Int.ofNat ptr.op.toFlat + (Buffed.Operation.Offsets.blockOperands (ptr.op.get! ctx)).toInt).toNat +
+  ptr.index * Buffed.BlockOperand.size.toNat
+
+def BlockArgumentPtr.toFlat (ptr : BlockArgumentPtr) :=
+  (Int.ofNat ptr.block.toFlat + Buffed.Block.Offsets.arguments.toInt).toNat +
+  ptr.index * Buffed.BlockArgument.size.toNat
+
+def ValuePtr.toFlat (ptr : ValuePtr) (ctx : IRContext OpInfo) :=
+  match ptr with
+  | .opResult ptr => ptr.toFlat ctx
+  | .blockArgument ptr => ptr.toFlat
+
+def OpOperandPtrPtr.toFlat (ptr : OpOperandPtrPtr) (ctx : IRContext OpInfo) :=
+  match ptr with
+  | .operandNextUse ptr => ptr.toFlat ctx
+  | .valueFirstUse ptr => ptr.toFlat ctx
+
+def BlockOperandPtrPtr.toFlat (ptr : BlockOperandPtrPtr) (ctx : IRContext OpInfo) :=
+  match ptr with
+  | .blockOperandNextUse ptr => ptr.toFlat ctx
+  | .blockFirstUse ptr => ptr.toFlat
+
+/-! ## A pointer is representable if it fits in 63 bits. -/
+
+@[grind] def OperationPtr.IsRepr (ptr : OperationPtr) : Prop :=
+  ptr.toFlat ≤ Int64.maxNatValue
+
+@[grind] def BlockPtr.IsRepr (ptr : BlockPtr) : Prop :=
+  ptr.toFlat ≤ Int64.maxNatValue
+
+@[grind] def RegionPtr.IsRepr (ptr : RegionPtr) : Prop :=
+  ptr.toFlat ≤ Int64.maxNatValue
+
+@[grind] def OpResultPtr.IsRepr (ctx : IRContext OpInfo) (ptr : OpResultPtr) : Prop :=
+  ptr.toFlat ctx ≤ Int64.maxNatValue
+
+@[grind] def OpOperandPtr.IsRepr (ctx : IRContext OpInfo) (ptr : OpOperandPtr) : Prop :=
+  ptr.toFlat ctx ≤ Int64.maxNatValue
+
+@[grind] def BlockOperandPtr.IsRepr (ctx : IRContext OpInfo) (ptr : BlockOperandPtr) : Prop :=
+  ptr.toFlat ctx ≤ Int64.maxNatValue
+
+@[grind] def BlockArgumentPtr.IsRepr (ptr : BlockArgumentPtr) : Prop :=
+  ptr.toFlat ≤ Int64.maxNatValue
+
+@[grind] def ValuePtr.IsRepr (ctx : IRContext OpInfo) (ptr : ValuePtr) : Prop :=
+  ptr.toFlat ctx ≤ Int64.maxNatValue
+
+@[grind] def OpOperandPtrPtr.IsRepr (ctx : IRContext OpInfo) (ptr : OpOperandPtrPtr) : Prop :=
+  ptr.toFlat ctx ≤ Int64.maxNatValue
+
+@[grind] def BlockOperandPtrPtr.IsRepr (ctx : IRContext OpInfo) (ptr : BlockOperandPtrPtr) : Prop :=
+  ptr.toFlat ctx ≤ Int64.maxNatValue
+
+/-! ## Translate a high-level pointer to a buffed address. -/
+
+def OperationPtr.toM (ptr : OperationPtr) : OperationMPtr := ptr.id.toUInt64
+def OperationPtr.toO (ptr : Option OperationPtr) : OperationOPtr :=
+  match ptr with
+  | some ptr => ptr.toM
+  | none => .none
+
+def BlockPtr.toM (ptr : BlockPtr) : BlockMPtr := ptr.id.toUInt64
+def BlockPtr.toO (ptr : Option BlockPtr) : BlockOPtr :=
+  match ptr with
+  | some ptr => ptr.toM
+  | none => .none
+
+def RegionPtr.toM (ptr : RegionPtr) : RegionMPtr := ptr.id.toUInt64
+def RegionPtr.toO (ptr : Option RegionPtr) : RegionOPtr :=
+  match ptr with
+  | some ptr => ptr.toM
+  | none => .none
+
+def OpResultPtr.toM (ptr : OpResultPtr) (ctx : IRContext OpInfo) : OpResultMPtr :=
+  (ptr.toFlat ctx).toUInt64
+def OpResultPtr.toO (ptr : Option OpResultPtr) (ctx : IRContext OpInfo) : OpResultOPtr :=
+  match ptr with
+  | some ptr => ptr.toM ctx
+  | none => .none
+
+def BlockArgumentPtr.toM (ptr : BlockArgumentPtr) : BlockArgumentMPtr :=
+  ptr.toFlat.toUInt64
+def BlockArgumentPtr.toO (ptr : Option BlockArgumentPtr) : BlockArgumentOPtr :=
+  match ptr with
+  | some ptr => ptr.toM
+  | none => .none
+
+def OpOperandPtr.toM (ptr : OpOperandPtr) (ctx : IRContext OpInfo) : OpOperandMPtr :=
+  (ptr.toFlat ctx).toUInt64
+def OpOperandPtr.toO (ptr : Option OpOperandPtr) (ctx : IRContext OpInfo) : OpOperandOPtr :=
+  match ptr with
+  | some ptr => ptr.toM ctx
+  | none => .none
+
+def BlockOperandPtr.toM (ptr : BlockOperandPtr) (ctx : IRContext OpInfo) : BlockOperandMPtr :=
+  (ptr.toFlat ctx).toUInt64
+def BlockOperandPtr.toO (ptr : Option BlockOperandPtr) (ctx : IRContext OpInfo) : BlockOperandOPtr :=
+  match ptr with
+  | some ptr => ptr.toM ctx
+  | none => .none
+
+def ValuePtr.toM (ptr : ValuePtr) (ctx : IRContext OpInfo) : ValueImplMPtr :=
+  (ptr.toFlat ctx).toUInt64
+def ValuePtr.toO (ptr : Option ValuePtr) (ctx : IRContext OpInfo) : ValueImplOPtr :=
+  match ptr with
+  | some ptr => ptr.toM ctx
+  | none => .none
+
+def OpOperandPtrPtr.toM (ptr : OpOperandPtrPtr) (ctx : IRContext OpInfo) : GenericMPtr :=
+  (ptr.toFlat ctx).toUInt64
+
+def BlockOperandPtrPtr.toM (ptr : BlockOperandPtrPtr) (ctx : IRContext OpInfo) : GenericMPtr :=
+  (ptr.toFlat ctx).toUInt64
+
+def GenericPtr.toM (ptr : GenericPtr) (ctx : IRContext OpInfo) : GenericMPtr :=
+  match ptr with
+  | .operation ptr => ptr.toM
+  | .block ptr => ptr.toM
+  | .region ptr => ptr.toM
+  | .opResult ptr => ptr.toM ctx
+  | .blockArgument ptr => ptr.toM
+  | .opOperand ptr => ptr.toM ctx
+  | .blockOperand ptr => ptr.toM ctx
+  | .blockOperandPtr ptr => ptr.toM ctx
+  | .value ptr => ptr.toM ctx
+  | .opOperandPtr ptr => ptr.toM ctx
+
+/-! ## Range of a pointer -/
+
+def OperationPtr.range (op : OperationPtr) (ctx : IRContext OpInfo) :=
+  op.toFlat + (Buffed.Operation.range op ctx)
+
+def BlockPtr.range (bl : BlockPtr) (ctx : IRContext OpInfo) :=
+  bl.toFlat + Buffed.Block.range bl ctx
+
+def RegionPtr.range (rg : RegionPtr) :=
+  rg.toFlat + Buffed.Region.range
+
+def OpResultPtr.range (res : OpResultPtr) (ctx : IRContext OpInfo) :=
+  res.toFlat ctx + Buffed.OpResult.range
+
+def BlockArgumentPtr.range (arg : BlockArgumentPtr) :=
+  arg.toFlat + Buffed.BlockArgument.range
+
+def OpOperandPtr.range (opr : OpOperandPtr) (ctx : IRContext OpInfo) :=
+  opr.toFlat ctx + Buffed.OpOperand.range
+
+def BlockOperandPtr.range (opr : BlockOperandPtr) (ctx : IRContext OpInfo) :=
+  opr.toFlat ctx + Buffed.BlockOperand.range
+
+def ValuePtr.range (val : ValuePtr) (ctx : IRContext OpInfo) :=
+  match val with
+  | .opResult res => res.range ctx
+  | .blockArgument arg => arg.range
+
+def OpOperandPtrPtr.range (ptr : OpOperandPtrPtr) (ctx : IRContext OpInfo) :=
+  match ptr with
+  | .operandNextUse opr => opr.range ctx
+  | .valueFirstUse val => val.range ctx
+
+def BlockOperandPtrPtr.range (ptr : BlockOperandPtrPtr) (ctx : IRContext OpInfo) :=
+  match ptr with
+  | .blockOperandNextUse opr => opr.range ctx
+  | .blockFirstUse bl => bl.range ctx
+
+def GenericPtr.range (ptr : GenericPtr) (ctx : IRContext OpInfo) : Std.Rco Nat :=
+  match ptr with
+  | .operation op => op.range ctx
+  | .block bl => bl.range ctx
+  | .region rg => rg.range
+  | .opResult res => res.range ctx
+  | .opOperand opr => opr.range ctx
+  | .blockOperand opr => opr.range ctx
+  | .blockOperandPtr ptr => ptr.range ctx
+  | .blockArgument arg => arg.range
+  | .value val => val.range ctx
+  | .opOperandPtr ptr => ptr.range ctx
+
+/-! ## An object is representable if all its fields are representable. -/
+
+@[grind]
+structure ValueImpl.IsRepr (val : ValueImpl) (ctx : IRContext OpInfo) where
+  firstUse : val.firstUse.maybe₁ (OpOperandPtr.IsRepr ctx)
+
+@[grind]
+structure OpResult.IsRepr (val : OpResult) (ctx : IRContext OpInfo) where
+  valueImpl : val.toValueImpl.IsRepr ctx
+  index : val.index ≤ UInt32.size
+  owner : val.owner.IsRepr
+
+@[grind]
+structure BlockArgument.IsRepr (val : BlockArgument) (ctx : IRContext OpInfo) where
+  valueImpl : val.toValueImpl.IsRepr ctx
+  index : val.index ≤ UInt32.size
+  owner : val.owner.IsRepr
+
+@[grind]
+structure OpOperand.IsRepr (val : OpOperand) (ctx : IRContext OpInfo) where
+  nextUse : val.nextUse.maybe₁ (OpOperandPtr.IsRepr ctx)
+  back : val.back.IsRepr ctx
+  owner : val.owner.IsRepr
+  value : val.owner.IsRepr
+
+@[grind]
+structure BlockOperand.IsRepr (val : BlockOperand) (ctx : IRContext OpInfo) where
+  nextUse : val.nextUse.maybe₁ (BlockOperandPtr.IsRepr ctx)
+  back : val.back.IsRepr ctx
+  owner : val.owner.IsRepr
+  value : val.owner.IsRepr
+
+@[grind]
+structure Operation.IsRepr (val : Operation OpInfo) (ctx : IRContext OpInfo) where
+  results : ∀ res ∈ val.results, res.IsRepr ctx
+  prev : val.prev.maybe₁ OperationPtr.IsRepr
+  next : val.next.maybe₁ OperationPtr.IsRepr
+  parent : val.parent.maybe₁ BlockPtr.IsRepr
+  blockOperands : ∀ bo ∈ val.blockOperands, bo.IsRepr ctx
+  regions : ∀ rg ∈ val.blockOperands, rg.IsRepr ctx
+  operands : ∀ operand ∈ val.blockOperands, operand.IsRepr ctx
+
+@[grind]
+structure Block.IsRepr (val : Block) (ctx : IRContext OpInfo) where
+  firstUse : val.firstUse.maybe₁ (BlockOperandPtr.IsRepr ctx)
+  prev : val.prev.maybe₁ BlockPtr.IsRepr
+  next : val.next.maybe₁ BlockPtr.IsRepr
+  parent : val.parent.maybe₁ RegionPtr.IsRepr
+  firstOp : val.firstOp.maybe₁ OperationPtr.IsRepr
+  lastOp : val.lastOp.maybe₁ OperationPtr.IsRepr
+  arguments : ∀ ba ∈ val.arguments, ba.IsRepr ctx
+
+@[grind]
+structure Region.IsRepr (val : Region) (ctx : IRContext OpInfo) where
+  firstBlock : val.firstBlock.maybe₁ BlockPtr.IsRepr
+  lastBlock : val.lastBlock.maybe₁ BlockPtr.IsRepr
+  parent : val.parent.maybe₁ OperationPtr.IsRepr
+
+@[grind]
+structure IRContext.IsRepr (ctx : IRContext OpInfo) where
+  operations op (hin : op ∈ ctx.operations) : (op.get! ctx).IsRepr ctx
+  blocks blk (hin : blk ∈ ctx.blocks) : (blk.get! ctx).IsRepr ctx
+  regions rg (hin : rg ∈ ctx.regions) : (rg.get! ctx).IsRepr ctx
+
+/-! ## Refinement predicate. -/
+
+structure OpResultPtr.Matches (ctx : IRContext OpInfo) (bctx : IRBufContext OpInfo) (res : OpResultPtr) where
+  ptr_repr : res.IsRepr ctx
+  obj_repr : (res.get! ctx).IsRepr ctx
+  type : bctx.attributes[(res.toM ctx).readType! bctx]? = some (res.get! ctx).type
+  firstUse : OpOperandPtr.toO (res.get! ctx).firstUse ctx = (res.toM ctx).readFirstUse! bctx
+  index : (res.get! ctx).index = ((res.toM ctx).readIndex! bctx).toNat
+  owner : (res.get! ctx).owner.toM = (res.toM ctx).readOwner! bctx
+
+structure BlockOperandPtr.Matches (ctx : IRContext OpInfo) (bctx : IRBufContext OpInfo) (res : BlockOperandPtr) where
+  ptr_repr : res.IsRepr ctx
+  obj_repr : (res.get! ctx).IsRepr ctx
+  nextUse : BlockOperandPtr.toO (res.get! ctx).nextUse ctx = BlockOperandMPtr.readNextUse! bctx (res.toM ctx)
+  back : ((res.get! ctx).back.toFlat ctx).toUInt64 = BlockOperandMPtr.readBack! bctx (res.toM ctx)
+  owner : (res.get! ctx).owner.toM = BlockOperandMPtr.readOwner! bctx (res.toM ctx)
+  value : (res.get! ctx).value.toM = BlockOperandMPtr.readValue! bctx (res.toM ctx)
+
+structure BlockArgumentPtr.Matches (ctx : IRContext OpInfo) (bctx : IRBufContext OpInfo) (arg : BlockArgumentPtr) where
+  ptr_repr : arg.IsRepr
+  obj_repr : (arg.get! ctx).IsRepr ctx
+  type : bctx.attributes[arg.toM.readType! bctx]? = some (arg.get! ctx).type
+  firstUse : OpOperandPtr.toO (arg.get! ctx).firstUse ctx = arg.toM.readFirstUse! bctx
+  index : (arg.get! ctx).index = (arg.toM.readIndex! bctx).toNat
+  owner : (arg.get! ctx).owner.toM = arg.toM.readOwner! bctx
+  -- `loc` is not implemented yet
+
+structure BlockPtr.Matches (ctx : IRContext OpInfo) (bctx : IRBufContext OpInfo) (res : BlockPtr) where
+  ptr_repr : res.IsRepr
+  obj_repr : (res.get! ctx).IsRepr ctx
+  firstUse : BlockOperandPtr.toO (res.get! ctx).firstUse ctx = BlockMPtr.readFirstUse! bctx (res.toM)
+  prev : BlockPtr.toO (res.get! ctx).prev = BlockMPtr.readPrev! bctx (res.toM)
+  next : BlockPtr.toO (res.get! ctx).next = BlockMPtr.readNext! bctx (res.toM)
+  parent : RegionPtr.toO (res.get! ctx).parent = BlockMPtr.readParent! bctx (res.toM)
+  firstOp : OperationPtr.toO (res.get! ctx).firstOp = BlockMPtr.readFirstOp! bctx (res.toM)
+  lastOp : OperationPtr.toO (res.get! ctx).lastOp = BlockMPtr.readLastOp! bctx (res.toM)
+  numArguments : (res.get! ctx).arguments.size = (BlockMPtr.readNumArguments! bctx (res.toM)).toNat
+  arguments idx (hidx : idx < (res.getNumArguments! ctx)) : (res.getArgument idx).Matches ctx bctx
+
+structure OpOperandPtr.Matches (ctx : IRContext OpInfo) (bctx : IRBufContext OpInfo) (res : OpOperandPtr) where
+  ptr_repr : res.IsRepr ctx
+  obj_repr : (res.get! ctx).IsRepr ctx
+  nextUse : OpOperandPtr.toO (res.get! ctx).nextUse ctx = OpOperandMPtr.readNextUse! bctx (res.toM ctx)
+  back : ((res.get! ctx).back.toFlat ctx).toUInt64 = OpOperandMPtr.readBack! bctx (res.toM ctx)
+  owner : (res.get! ctx).owner.toM = OpOperandMPtr.readOwner! bctx (res.toM ctx)
+  value : (res.get! ctx).value.toM ctx = OpOperandMPtr.readValue! bctx (res.toM ctx)
+
+structure RegionPtr.Matches (ctx : IRContext OpInfo) (bctx : IRBufContext OpInfo) (reg : RegionPtr) where
+  ptr_repr : reg.IsRepr
+  obj_repr : (reg.get! ctx).IsRepr ctx
+  firstBlock : BlockPtr.toO (reg.get! ctx).firstBlock = RegionMPtr.readFirstBlock! bctx (reg.toM)
+  lastBlock : BlockPtr.toO (reg.get! ctx).lastBlock = RegionMPtr.readLastBlock! bctx (reg.toM)
+  parent : OperationPtr.toO (reg.get! ctx).parent = RegionMPtr.readParent! bctx (reg.toM)
+
+structure OperationPtr.Matches (ctx : IRContext OpInfo) (bctx : IRBufContext OpInfo) (op : OperationPtr) where
+  ptr_repr : op.IsRepr
+  obj_repr : (op.get! ctx).IsRepr ctx
+  results res (hin : res ∈ (op.getOpResults! ctx)) : res.Matches ctx bctx
+  prev : OperationPtr.toO (op.get! ctx).prev = op.toM.readPrev! bctx
+  next : OperationPtr.toO (op.get! ctx).next = op.toM.readNext! bctx
+  parent : BlockPtr.toO (op.get! ctx).parent = op.toM.readParent! bctx
+  opType : (op.get! ctx).opType = Operation.decodeOpInfo (op.toM.readOpType! bctx)
+  attrs : bctx.attributes[op.toM.readAttrs! bctx]? = some (op.get! ctx).attrs
+  -- TODO: properties
+  numBlockOperands : op.getNumSuccessors! ctx = (op.toM.readNumBlockOperands! bctx).toNat
+  blockOperands bo (hin : bo ∈ (op.getSuccessors! ctx)) : bo.Matches ctx bctx
+  numRegions : op.getNumRegions! ctx = (op.toM.readNumRegions! bctx).toNat
+  regions idx (hidx : idx < (op.getNumRegions! ctx)) : (op.getRegion! ctx idx).Matches ctx bctx
+  numOperands : op.getNumOperands! ctx = (op.toM.readNumOperands! bctx).toNat
+  operands idx (hidx : idx < (op.getNumOperands! ctx)) : (op.getOpOperand idx).Matches ctx bctx
+
+def GenericPtr.MayOverlap (ptr₁ ptr₂ : GenericPtr) : Prop :=
+  match ptr₁, ptr₂ with
+  | .operation ptr₁, .opOperand ptr₂ => ptr₁ = ptr₂.op
+  | .opOperand ptr₁, .operation ptr₂ => ptr₁.op = ptr₂
+  | .operation ptr₁, .opResult ptr₂ => ptr₁ = ptr₂.op
+  | .opResult ptr₁, .operation ptr₂ => ptr₁.op = ptr₂
+  | .blockOperand ptr₁, .operation ptr₂ => ptr₁.op = ptr₂
+  | .operation ptr₁, .blockOperand ptr₂ => ptr₁ = ptr₂.op
+  | .block ptr₁, .blockArgument ptr₂ => ptr₁ = ptr₂.block
+  | .blockArgument ptr₁, .block ptr₂ => ptr₁.block = ptr₂
+  | _, _ => False
+
+@[grind]
+structure Sim (bctx : IRBufContext OpInfo) (ctx : IRContext OpInfo) where
+  /-- All the values are representable. -/
+  repr : ctx.IsRepr
+  /-- Allocated addresses do not go beyond the buffer size. -/
+  in_bounds (ptr : GenericPtr) (ib : ptr.InBounds ctx) :
+    IsIncluded (ptr.range ctx) bctx.mem.range
+  /-- The allocations are disjoint. -/
+  disjoint_allocs (ptr₁ ptr₂ : GenericPtr) (ib₁ : ptr₁.InBounds ctx) (ib₂ : ptr₂.InBounds ctx)
+      (h : ¬ ptr₁.MayOverlap ptr₂) (hneq : ptr₁ ≠ ptr₂) :
+    IsDisjoint (ptr₁.range ctx) (ptr₂.range ctx)
+  /-- The buffer contains the encodings of all the operations. -/
+  encoding_op (op : OperationPtr) (ib : op.InBounds ctx) :
+    op.Matches ctx bctx
+  /-- The buffer contains the encodings of all the blocks. -/
+  encoding_block (blk : BlockPtr) (ib : blk.InBounds ctx) :
+    blk.Matches ctx bctx
+  /-- The buffer contains the encodings of all the regions. -/
+  encoding_region (rg : RegionPtr) (ib : rg.InBounds ctx) :
+    rg.Matches ctx bctx
+
+structure Sim.IRContext where
+  buf : IRBufContext OpInfo
+  ctx : Veir.IRContext OpInfo
+  sim : Sim buf ctx
